---
{"dg-publish":true,"dg-path":"academia/CSC110/01 Course Notes/7 Number Theory/7.4 Modular Arithmetic.md","permalink":"/academia/csc-110/01-course-notes/7-number-theory/7-4-modular-arithmetic/","created":"2023-10-25T13:57:35.334-04:00","updated":"2023-11-06T00:02:45.900-05:00"}
---

#CSC110  

**Covered in:**
- [[100 ðŸ“’ Academia/CSC110/02 Lecture Notes/Lecture 17 Modular Arithmetic\|Lecture 17 Modular Arithmetic]]

Recall from [[100 ðŸ“’ Academia/CSC110/01 Course Notes/7 Number Theory/7.1 Introduction to Number Theory\|7.1 Introduction to Number Theory]].

> [!note] *Definition.*
> Let $a,b,n \in \mathbb{Z}$, and assume $n \neq 0$. We say that $a$ **is equivalent to $b$ modulo $n$** when $n \mid a - b$.
> $$a \equiv b \pmod{n}$$

> [!note] **Theorem.**
> For all $a,b,c,d,n \in \mathbb{Z}$, if $n \neq 0$, $a \equiv c \pmod{n}$, and $b \equiv d \pmod{n}$, then:
> 1. $a + b \equiv c + d \pmod{n}$
> 2. $a - b \equiv c - d \pmod{n}$
> 3. $ab \equiv cd \pmod{n}$

Prove (2).
$$\forall a,b,c,d,n \in \mathbb{Z}, (n \neq 0 \; \land \; (n \mid a - c) \; \land \; (n \mid b - d)) \implies n \mid (a-b)-(c-d)$$
*Proof.*
Let $a,b,c,d,n \in \mathbb{Z}$.
Assume that $n \neq 0$, $n \mid a - c$, and that $n \mid b - d$.
By the Divisibility of Linear Combinations Theorem, since $n \mid (a-c)$ and $n \mid (b-d)$, it divides their difference.
$$\begin{aligned}
n \mid (a - c) - (b - d)\\
n \mid (a - b) - (c - d)
\end{aligned}$$
<div class="right-align"> <span class="math display">\blacksquare</span></div>

# Modular division

- A false theorem:
	- $\forall a,b,k,n \in \mathbb{Z}, n \neq 0 \land ak \equiv bk \pmod{n} \implies a \equiv b \pmod{n}$

<br>

> [!note] Theorem. (*Modular inverse*)
> Let $n \in \mathbb{Z}^{+}$ and $a \in \mathbb{Z}$. If $\text{gcd}(a,n) = 1$, then there exists $p \in \mathbb{Z}$ such that $ap \equiv 1 \pmod{n}$
> - We say that $p$ is a **modular inverse of $a$ modulo $n$**
{ #c5c63b}


$$\forall n \in \mathbb{Z}^{+}, \forall a \in \mathbb{Z}, \text{gcd}(a,n) = 1 \implies (\exists p \in \mathbb{Z}, ap \equiv 1 \pmod{n})$$
*Proof.*
Let $n \in \mathbb{Z}^{+}$ and $a \in \mathbb{Z}$. Assume $\text{gcd}(a,n) = 1$.
We want to show that $n \mid ap - 1$, so there exists an integer $k$ such that $ap - 1 = nk$.
Since $\text{gcd}(a,n) = 1$, by the *GCD Characterization Theorem*, we know that there exists integers $p$ and $q$ such that $1 = pa + qn$.
Take $k = -q$.
$$\begin{align*}
1 &= pa + qn\\
1 - pa &= qn\\
pa - 1 &= (-q)n\\
ap - 1 &= kn\\
n &\mid ap - 1 && \text{(by definition of divisibility)}\\
ap &\equiv 1 \pmod{n} && \text{(by definition of modular equivalence)}
\end{align*}$$
<div class="right-align"> 
<span class="math display">\blacksquare</span>
</div>


> [!note] 
> **Theorem.** (Modular division)
> Let $a \in \mathbb{Z}$ and $n \in \mathbb{Z}^{+}$.
> If $\text{gcd}(a,n)=1$, then for all $b \in \mathbb{Z}$, there exists $k \in \mathbb{Z}$ such that $ak \equiv b \pmod{n}$.

$$\forall n \in \mathbb{Z}^{+}, \forall a \in \mathbb{Z}, \text{gcd}(a,n) = 1 \implies (\forall b \in \mathbb{Z}, \exists k \in \mathbb{Z}, ak \equiv b \pmod{n})$$
*Proof.*
Let $n \in \mathbb{Z}^{+}$ and $a \in \mathbb{Z}$. 
Assume $\text{gcd}(a,n) = 1$, and let $b \in \mathbb{Z}$.
We want to show that there exists $k \in \mathbb{Z}$ such that $ak \equiv b \pmod{n}$.

From the [[100 ðŸ“’ Academia/CSC110/01 Course Notes/7 Number Theory/7.4 Modular Arithmetic#^c5c63b\|Modular Inverses]] Theorem, we know that there exists $p \in \mathbb{Z}$ such that $ap \equiv 1 \pmod{1}$ (since our assumption is $\text{gcd}(a,n) = 1$).
Take $k = pb$.
$$\begin{align*}
ap &\equiv 1 \pmod{1}\\
apb &\equiv b \pmod{n}\\
ak &\equiv b \pmod{n}
\end{align*}$$
<div class="right-align"> <span class="math display">\blacksquare</span> </div>
